cacheIfScript.sml
@@ -9,60 +9,88 @@ val _ = new_theory "cacheIf";
 
 (* dummy cache for now *)
 
+val _ = Datatype `line = CLINE word`;
+
+val line_neq_lem = store_thm("line_neq_lem", ``
+!l1 l2. l1 <> l2 ==> ?w1 w2. (l1 = CLINE w1) /\ (l2 = CLINE w2) /\ w1 <> w2
+``,
+  Cases >> Cases >> METIS_TAC []
+);
+
+val the_line_def = Define `the_line (CLINE w) = w`;
+
+val _ = Parse.type_abbrev("tag", ``:bool[30]``);
+
+val _ = Parse.type_abbrev("line_view", ``:bool -> tag -> word``);
+
 val _ = Parse.type_abbrev("cache_state", 
-			  ``:padr -> (word # bool) option``);
+			  ``:tag -> (line # bool) option``);
+
+val tag_def = Define `tag (pa:padr) = the_adr pa`;
+
+val lv_def = Define `lv (mv:mem_view) c (pa:padr) = CLINE (mv c pa)`;
+
+val lw_def = Define `lw l (pa:padr) = the_line l`;
+
+val lu_def = Define `lu (l:line) (pa:padr) (w:word) = CLINE w`;
 
 val hit_def = Define `
    (hit NONE = F)
-/\ (hit (SOME (w:word,d:bool)) = T)
+/\ (hit (SOME (w:line,d:bool)) = T)
 `;
 
-val dirty_def = Define `
-   (dirty NONE = F)
-/\ (dirty (SOME (w:word,d:bool)) = d)
+val dirty__def = Define `
+   (dirty_ NONE = F)
+/\ (dirty_ (SOME (w:line,d:bool)) = d)
 `;
 
 val dirty_hit_lem = store_thm("dirty_hit_lem", ``
-!l. dirty l ==> hit l
+!l. dirty_ l ==> hit l
 ``,
-  Cases >- ( RW_TAC std_ss [dirty_def, hit_def] ) >>
+  Cases >- ( RW_TAC std_ss [dirty__def, hit_def] ) >>
   `?w d. x = (w,d)` by ( RW_TAC std_ss [pairTheory.pair_CASES] ) >>
-  RW_TAC std_ss [dirty_def, hit_def]
+  RW_TAC std_ss [dirty__def, hit_def]
 );
 
 val not_hit_not_dirty_lem = 
 dirty_hit_lem |> SPEC_ALL |> (CONV_RULE CONTRAPOS_CONV) |> GEN_ALL;
 
 val cnt_def = Define `
-   (cnt (SOME (w:word,d:bool)) = w)
+   (cnt (SOME (w:line,d:bool)) = w)
 `;
 
-val chit_def = Define `chit_ (ca:cache_state) pa = hit (ca pa)`;
+val chit_def = Define `chit_ (ca:cache_state) (pa:padr) = hit (ca (tag pa))`;
 
-val cdirty_def = Define `cdirty_ (ca:cache_state) pa = dirty (ca pa)`;
+val ldirty_def = Define `ldirty_ (ca:cache_state) t = 
+dirty_ (ca t)`;
+val cdirty_def = Define `cdirty_ (ca:cache_state) (pa:padr) = 
+dirty_ (ca (tag pa))`;
 
 val not_cdirty_lem = store_thm("not_cdirty_lem", ``
-!ca pa. ~cdirty_ ca pa <=> ((?w. ca pa = SOME (w,F)) \/ (ca pa = NONE))
+!ca pa. ~cdirty_ ca pa <=> (    (?w. ca (tag pa) = SOME (w,F)) 
+			     \/ (ca (tag pa) = NONE))
 ``,
   RW_TAC std_ss [cdirty_def] >>
-  Cases_on `ca pa`
+  Cases_on `ca (tag pa)`
   >| [(* NONE *)
-      RW_TAC std_ss [dirty_def]
+      RW_TAC std_ss [dirty__def]
       ,
       (* SOME x *)
       `?v d. x = (v,d)` by ( METIS_TAC [pairTheory.pair_CASES] ) >>
-      RW_TAC std_ss [dirty_def]
+      RW_TAC std_ss [dirty__def]
      ]
 );
 
-val ccnt_def = Define `ccnt_ (ca:cache_state) pa = cnt (ca pa)`;
+val lcnt_def = Define `lcnt_ (ca:cache_state) t = cnt (ca t)`;
+val ccnt_def = Define `ccnt_ (ca:cache_state) pa = cnt (ca (tag pa))`;
+val ccntw_def = Define `ccntw_ (ca:cache_state) pa = lw (ccnt_ ca pa) pa`;
 
 (* add other properties of eviction policy here *)
 val evpol_exists = prove(``
-?evpol:cache_state -> padr -> padr option.
-!ca pa. evpol ca pa <> SOME pa
+?evpol:cache_state -> padr -> tag option.
+!ca pa pa'. (tag pa' = tag pa) ==> evpol ca pa <> SOME (tag pa')
 ``,
-  EXISTS_TAC ``\c:cache_state a:padr. NONE:padr option`` >>
+  EXISTS_TAC ``\c:cache_state a:padr. NONE:tag option`` >>
   RW_TAC std_ss []
 );
 
@@ -70,9 +98,9 @@ val evpol_spec = new_specification("evpol_spec",["evpol"], evpol_exists);
 
 val evict_def = Define `
    (evict ca NONE = (ca, NONE))
-/\ (evict ca (SOME pa') = ((pa' =+ NONE) ca, 
-			   if cdirty_ ca pa' 
-			   then SOME (pa', ccnt_ ca pa')
+/\ (evict ca (SOME t) = ((t =+ NONE) ca, 
+			   if ldirty_ ca t 
+			   then SOME (t, lcnt_ ca t)
 			   else NONE))
 `;
 
@@ -81,22 +109,22 @@ cfill ca (mv:mem_view) pa ev =
     if chit_ ca pa 
     then evict ca ev
     else let (ca', wb) = evict ca ev 
-	 in ((pa =+ SOME (mv T pa,F)) ca', wb)
+	 in (((tag pa) =+ SOME ((lv mv T pa),F)) ca', wb)
 `;
 
 val cevict_def = Define `
    (cevict ca NONE = ca)
-/\ (cevict ca (SOME pa) = (pa =+ NONE) ca)
+/\ (cevict ca (SOME t) = (t =+ NONE) ca)
 `;
 
 val cevict_self_lem = store_thm("cevict_self_lem", ``
-!ca pa. (cevict ca (evpol ca pa)) pa = ca pa
+!ca pa. (cevict ca (evpol ca pa)) (tag pa) = ca (tag pa)
 ``,
   REPEAT STRIP_TAC >> 
   Cases_on `evpol ca pa` >> (
       RW_TAC std_ss [cevict_def]
   ) >>
-  `x <> pa` by ( METIS_TAC [evpol_spec] ) >>
+  `x <> tag pa` by ( METIS_TAC [evpol_spec] ) >>
   RW_TAC std_ss [combinTheory.UPDATE_APPLY]
 );
 
@@ -104,12 +132,12 @@ val cfill_ca_def = Define `
 cfill_ca ca (mv:mem_view) pa ev = 
     if chit_ ca pa 
     then (cevict ca ev)
-    else (pa =+ SOME (mv T pa,F)) (cevict ca ev)
+    else (tag pa =+ SOME (lv mv T pa,F)) (cevict ca ev)
 `;
 
 val levict_def = Define `
    (levict ca NONE = NONE)
-/\ (levict ca (SOME pa) = if cdirty_ ca pa then SOME (pa, ccnt_ ca pa) else NONE)
+/\ (levict ca (SOME t) = if ldirty_ ca t then SOME (t, lcnt_ ca t) else NONE)
 `; 
 
 val cfill_lem = store_thm("cfill_lem", ``
@@ -124,21 +152,21 @@ val cfill_lem = store_thm("cfill_lem", ``
 val ctf_def = Define `
    (ctf ca mv (RD pa T)   = cfill ca mv pa (evpol ca pa))
 /\ (ctf ca mv (WT pa w T) = let (ca',wb) = cfill ca mv pa (evpol ca pa)
-			    in ((pa =+ SOME (w,T)) ca', wb))
-/\ (ctf ca mv (CL pa)     = ((pa =+ NONE) ca, levict ca (SOME pa)))
+			    in ((tag pa =+ SOME (CLINE w,T)) ca', wb))
+/\ (ctf ca mv (CL pa)     = ((tag pa =+ NONE) ca, levict ca (SOME (tag pa))))
 `;
 
 val ctf_ca_def = Define `
    (ctf_ca ca mv (RD pa T)   = cfill_ca ca mv pa (evpol ca pa))
-/\ (ctf_ca ca mv (WT pa w T) = (pa =+ SOME (w,T)) 
+/\ (ctf_ca ca mv (WT pa w T) = (tag pa =+ SOME (CLINE w,T)) 
 				   (cfill_ca ca mv pa (evpol ca pa)))
-/\ (ctf_ca ca mv (CL pa)     = (pa =+ NONE) ca)
+/\ (ctf_ca ca mv (CL pa)     = (tag pa =+ NONE) ca)
 `;
 
 val ctf_wb_def = Define `
-   (ctf_wb ca mv (RD pa T)   = levict ca (evpol ca pa))
+   (ctf_wb ca (mv:mem_view) (RD pa T)   = levict ca (evpol ca pa))
 /\ (ctf_wb ca mv (WT pa w T) = levict ca (evpol ca pa))
-/\ (ctf_wb ca mv (CL pa)     = levict ca (SOME pa))
+/\ (ctf_wb ca mv (CL pa)     = levict ca (SOME (tag pa)))
 `;
 
 val ctf_lem = store_thm("ctf_lem", ``
@@ -150,20 +178,20 @@ val ctf_lem = store_thm("ctf_lem", ``
 );
 
 val ctf_ca_rd_lem = store_thm("ctf_ca_rd_lem", ``
-!ca mv dop pa. rd dop /\ CA dop ==> 
-    ((ctf_ca ca mv dop) pa = if pa = PA dop 
-			     then (if chit_ ca pa 
-				   then ca pa
-				   else SOME (mv T pa,F))
-			     else (if (evpol ca (PA dop) = SOME pa)
-				   then NONE
-			           else ca pa))
+!ca mv dop t. rd dop /\ CA dop ==> 
+    ((ctf_ca ca mv dop) t = if t = tag (PA dop)
+			    then (if hit (ca t) 
+				  then ca t
+				  else SOME (lv mv T (PA dop),F))
+			    else (if (evpol ca (PA dop) = SOME t)
+				  then NONE
+			          else ca t))
 ``,
   REPEAT STRIP_TAC >>
   `?pa'. dop = RD pa' T` by ( METIS_TAC [rd_CA_lem] ) >>
   FULL_SIMP_TAC std_ss [] >>
   RW_TAC std_ss [PA_def, ctf_ca_def, cfill_ca_def, 
-		 combinTheory.UPDATE_APPLY, cevict_def] >- (
+		 combinTheory.UPDATE_APPLY, cevict_def, chit_def] >- (
       RW_TAC std_ss [cevict_self_lem]
   ) >> (
       Cases_on `evpol ca pa'`
@@ -179,18 +207,18 @@ val ctf_ca_rd_lem = store_thm("ctf_ca_rd_lem", ``
 
 
 val ctf_ca_wt_lem = store_thm("ctf_ca_wt_lem", ``
-!ca mv dop pa. wt dop /\ CA dop ==> 
-    ((ctf_ca ca mv dop) pa = if pa = PA dop 
-			     then SOME (VAL dop,T)
-			     else (if evpol ca (PA dop) = SOME pa
-				   then NONE
-			           else ca pa))
+!ca mv dop t. wt dop /\ CA dop ==> 
+    ((ctf_ca ca mv dop) t = if t = tag (PA dop)
+			    then SOME (CLINE (VAL dop),T)
+			    else (if evpol ca (PA dop) = SOME t
+				  then NONE
+			          else ca t))
 ``,
   REPEAT STRIP_TAC >>
   `?pa' w. dop = WT pa' w T` by ( METIS_TAC [wt_CA_lem] ) >>
   FULL_SIMP_TAC std_ss [] >>
   RW_TAC std_ss [PA_def, ctf_ca_def, cfill_ca_def, 
-		 combinTheory.UPDATE_APPLY, cevict_def, VAL_def] >> (
+		 combinTheory.UPDATE_APPLY, cevict_def, VAL_def, chit_def] >> (
       Cases_on `evpol ca pa'`
       >| [(* evict NONE *)
           RW_TAC std_ss [cevict_def]
@@ -203,9 +231,9 @@ val ctf_ca_wt_lem = store_thm("ctf_ca_wt_lem", ``
 );
 
 val ctf_ca_cl_lem = store_thm("ctf_ca_cl_lem", ``
-!ca mv dop pa. cl dop ==> ((ctf_ca ca mv dop) pa = if pa = PA dop 
-						   then NONE 
-						   else ca pa)
+!ca mv dop t. cl dop ==> ((ctf_ca ca mv dop) t = if t = tag (PA dop)
+						 then NONE 
+						 else ca t)
 ``,
   REPEAT STRIP_TAC >>
   FULL_SIMP_TAC std_ss [cl_lem] >>
@@ -215,9 +243,9 @@ val ctf_ca_cl_lem = store_thm("ctf_ca_cl_lem", ``
 );
 
 val ctf_ca_evict_other_lem = store_thm("ctf_ca_evict_other_lem", ``
-!ca mv dop pa. CA dop /\ pa <> PA dop /\ 
-	       (cl dop \/ (evpol ca (PA dop) <> SOME pa)) ==>
-    ((ctf_ca ca mv dop) pa = ca pa)
+!ca mv dop t. CA dop /\ t <> tag (PA dop) 
+           /\ (cl dop \/ (evpol ca (PA dop) <> SOME t)) ==>
+    ((ctf_ca ca mv dop) t = ca t)
 ``,
   REPEAT GEN_TAC >>
   MATCH_MP_TAC (prove(``(A /\ B /\ (C \/ ~C /\ D) ==> E)
@@ -230,9 +258,9 @@ val ctf_ca_evict_other_lem = store_thm("ctf_ca_evict_other_lem", ``
 );
 
 val ctf_ca_evict_lem = store_thm("ctf_ca_evict_lem", ``
-!ca mv dop pa. CA dop /\ ~cl dop /\ pa <> PA dop 
-            /\ (evpol ca (PA dop) = SOME pa) ==>
-    ((ctf_ca ca mv dop) pa = NONE)
+!ca mv dop t. CA dop /\ ~cl dop /\ t <> tag (PA dop)
+           /\ (evpol ca (PA dop) = SOME t) ==>
+    ((ctf_ca ca mv dop) t = NONE)
 ``,
   REPEAT STRIP_TAC >>
   FULL_SIMP_TAC std_ss [not_cl_lem] >> (
@@ -241,13 +269,13 @@ val ctf_ca_evict_lem = store_thm("ctf_ca_evict_lem", ``
 );
 
 val ctf_wb_not_cl_lem = store_thm("ctf_wb_not_cl_lem", ``
-!ca mv dop pa. CA dop /\ ~cl dop ==> 
+!ca mv dop. CA dop /\ ~cl dop ==> 
     (ctf_wb ca mv dop = if evpol ca (PA dop) = NONE
 			then NONE 
-			else (if cdirty_ ca (THE (evpol ca (PA dop))) /\
-                                 THE (evpol ca (PA dop)) <> PA dop
+			else (if ldirty_ ca (THE (evpol ca (PA dop))) /\
+                                 THE (evpol ca (PA dop)) <> tag (PA dop)
 			      then SOME(THE (evpol ca (PA dop)), 
-					ccnt_ ca (THE(evpol ca (PA dop))))
+					lcnt_ ca (THE(evpol ca (PA dop))))
 			      else NONE))
 ``,
   REPEAT STRIP_TAC >>
@@ -271,20 +299,21 @@ val ctf_wb_not_cl_lem = store_thm("ctf_wb_not_cl_lem", ``
 val ctf_wb_cl_lem = store_thm("ctf_wb_cl_lem", ``
 !ca mv dop. cl dop ==> 
     (ctf_wb ca mv dop = if cdirty_ ca (PA dop) 
-			then SOME (PA dop, ccnt_ ca (PA dop)) 
+			then SOME (tag (PA dop), cnt (ca (tag (PA dop)))) 
                         else NONE)
 ``,
   REPEAT STRIP_TAC >>
   FULL_SIMP_TAC std_ss [cl_lem] >> 
-  RW_TAC std_ss [PA_def, ctf_wb_def, levict_def] 
+  RW_TAC std_ss [PA_def, ctf_wb_def, levict_def, cdirty_def, 
+		 lcnt_def, ldirty_def] 
 );
 
 
 val chit_lem = store_thm("chit_lem", ``
-!ca pa. chit_ ca pa <=> ?w d. ca pa = SOME (w,d)
+!ca pa. chit_ ca pa <=> ?w d. ca (tag pa) = SOME (w,d)
 ``,
   RW_TAC std_ss [chit_def] >>
-  Cases_on `ca pa` 
+  Cases_on `ca (tag pa)` 
   >| [(* case: NONE *)
       RW_TAC std_ss [hit_def]
       , 
@@ -297,10 +326,10 @@ val chit_lem = store_thm("chit_lem", ``
 );
 
 val not_chit_lem = store_thm("not_chit_lem", ``
-!ca pa. ~chit_ ca pa <=> (ca pa = NONE)
+!ca pa. ~chit_ ca pa <=> (ca (tag pa) = NONE)
 ``,
   RW_TAC std_ss [chit_def] >>
-  Cases_on `ca pa` 
+  Cases_on `ca (tag pa)` 
   >| [(* case: NONE *)
       RW_TAC std_ss [hit_def]
       , 
@@ -313,7 +342,7 @@ val not_chit_lem = store_thm("not_chit_lem", ``
 );
 
 val cfill_chit_ = store_thm("cfill_chit_", ``
-!ca mv pa x ca' y. ((ca', y) = cfill ca mv pa x) /\ (x <> SOME pa) ==>
+!ca mv pa x ca' y. ((ca', y) = cfill ca mv pa x) /\ (x <> SOME (tag pa)) ==>
     chit_ ca' pa					     
 ``,
   RW_TAC std_ss [chit_lem] >>
@@ -331,36 +360,137 @@ val cfill_chit_ = store_thm("cfill_chit_", ``
   )
 );
 
+
+(* memory cache line write-back and lookup *)
+
+val mlwb_def = Define `mlwb m (t:tag) (CLINE w) = (PADR t =+ w) m`;
+
+(* fetch line corresponding to pa according to line size *)
+val mllu_def = Define `mllu m pa = CLINE (m pa)`;
+
 (* proof obligations on the cache model, imported by generalized model *)
 
+val mlwb_oblg = store_thm("mlwb_oblg", ``
+!m t l pa. (tag pa = t) ==> (mlwb m t l pa = lw l pa)  
+``,
+  Cases_on `l` >>
+  RW_TAC std_ss [mlwb_def, lw_def, tag_def] >>
+  Cases_on `pa` >>
+  RW_TAC std_ss [the_adr_def, the_line_def, combinTheory.UPDATE_APPLY]
+); 
+
+val mlwb_other_oblg = store_thm("mlwb_other_oblg", ``
+!m t l pa. (tag pa <> t) ==> (mlwb m t l pa = m pa)  
+``,
+  Cases_on `l` >>
+  RW_TAC std_ss [mlwb_def, tag_def] >>
+  Cases_on `pa` >>
+  FULL_SIMP_TAC std_ss [the_adr_def] >>
+  RW_TAC std_ss [combinTheory.UPDATE_APPLY]
+); 
+
+val mllu_oblg = store_thm("mllu_oblg", ``
+!m pa pa'. (tag pa = tag pa') ==> (lw (mllu m pa') pa = m pa)  
+``,
+  RW_TAC std_ss [mllu_def, lw_def, tag_def] >>
+  Cases_on `pa` >>
+  Cases_on `pa'` >>
+  FULL_SIMP_TAC std_ss [the_adr_def, the_line_def]
+); 
+
+val tag_oblg = store_thm("tag_oblg", ``
+!t. ?pa. t = tag pa
+``,
+  RW_TAC std_ss [tag_def] >>
+  EXISTS_TAC ``PADR t`` >>
+  RW_TAC std_ss [the_adr_def]
+);
+
 val chit_oblg = store_thm("chit_oblg", ``
-!pa ca ca'. (ca pa = ca' pa) ==> (chit_ ca pa <=> chit_ ca' pa)
+!pa ca ca'. (ca (tag pa) = ca' (tag pa)) ==> (chit_ ca pa <=> chit_ ca' pa)
+``,
+  RW_TAC std_ss [chit_def]
+);
+
+val chit_other_oblg = store_thm("chit_other_oblg", ``
+!pa pa' ca. (tag pa = tag pa') ==> (chit_ ca pa <=> chit_ ca pa')
 ``,
   RW_TAC std_ss [chit_def]
 );
 
 val ccnt_oblg = store_thm("ccnt_oblg", ``
-!pa ca ca'. (ca pa = ca' pa) ==> (ccnt_ ca pa = ccnt_ ca' pa)
+!pa ca ca'. (ca (tag pa) = ca' (tag pa)) ==> (ccnt_ ca pa = ccnt_ ca' pa)
 ``,
   RW_TAC std_ss [ccnt_def]
 );
 
+val ccnt_other_oblg = store_thm("ccnt_other_oblg", ``
+!pa pa' ca. (tag pa = tag pa') ==> (ccnt_ ca pa = ccnt_ ca pa')
+``,
+  RW_TAC std_ss [ccnt_def]
+);
+
+val ccntw_oblg = store_thm("ccntw_oblg", ``
+!pa ca ca'. (ca (tag pa) = ca' (tag pa)) ==> (ccntw_ ca pa = ccntw_ ca' pa)
+``,
+  RW_TAC std_ss [ccntw_def] >>
+  IMP_RES_TAC ccnt_oblg >>
+  ASM_REWRITE_TAC []
+);
+
+val ccntw_ccnt_oblg = store_thm("ccntw_ccnt_oblg", ``
+!pa ca ca'. chit_ ca pa /\ chit_ ca' pa /\ (ccnt_ ca pa = ccnt_ ca' pa) ==> 
+    (ccntw_ ca pa = ccntw_ ca' pa)
+``,
+  RW_TAC std_ss [ccntw_def, ccnt_def] >>
+  IMP_RES_TAC chit_lem >>
+  FULL_SIMP_TAC std_ss [cnt_def]
+);
+
+val ccntw_ccnt_other_oblg = store_thm("ccntw_ccnt_other_oblg", ``
+!pa ca ca'. chit_ ca pa /\ chit_ ca' pa /\ (ccnt_ ca pa = ccnt_ ca' pa) ==> 
+    !pa'. (tag pa' = tag pa) ==> (ccntw_ ca pa' = ccntw_ ca' pa')
+``,
+  RW_TAC std_ss [ccntw_def, ccnt_def] >>
+  IMP_RES_TAC chit_lem >>
+  FULL_SIMP_TAC std_ss [cnt_def]
+);
+
+val ccntw_ccnt_diff_oblg = store_thm("ccntw_ccnt_diff_oblg", ``
+!pa ca ca'. chit_ ca pa /\ chit_ ca' pa /\ (ccnt_ ca pa <> ccnt_ ca' pa) ==> 
+    ?pa'. (tag pa' = tag pa) /\ (ccntw_ ca pa' <> ccntw_ ca' pa')
+``,
+  RW_TAC std_ss [ccntw_def, ccnt_def] >>
+  IMP_RES_TAC chit_lem >>
+  FULL_SIMP_TAC std_ss [cnt_def] >>
+  EXISTS_TAC ``pa:padr`` >>
+  RW_TAC std_ss [cnt_def, lw_def] >>
+  IMP_RES_TAC line_neq_lem >>
+  RW_TAC std_ss [the_line_def]
+);
+
+val ccnt_lcnt_oblg = store_thm("ccnt_lcnt_oblg", ``
+!ca pa. ccnt_ ca pa = lcnt_ ca (tag pa)
+``,
+  RW_TAC std_ss [ccnt_def, lcnt_def]
+);
+
 val ccnt_not_eq_oblg = store_thm("ccnt_not_eq_oblg", ``
 !pa ca ca'. chit_ ca pa /\ chit_ ca' pa /\ (cdirty_ ca pa <=> cdirty_ ca' pa)
-         /\ (ca pa <> ca' pa) ==> 
+         /\ (ca (tag pa) <> ca' (tag pa)) ==> 
     (ccnt_ ca pa <> ccnt_ ca' pa)
 ``,
   RW_TAC std_ss [ccnt_def] >>
   FULL_SIMP_TAC std_ss [chit_lem, cdirty_def] >>
   RW_TAC std_ss [cnt_def] >>
-  REV_FULL_SIMP_TAC std_ss [dirty_def]
+  REV_FULL_SIMP_TAC std_ss [dirty__def]
 );
 
 val miss_oblg = store_thm("miss_oblg", ``
-!ca pa. ~chit_ ca pa <=> (ca pa = NONE)
+!ca pa. ~chit_ ca pa <=> (ca (tag pa) = NONE)
 ``,
   RW_TAC std_ss [chit_def] >>
-  Cases_on `ca pa` 
+  Cases_on `ca (tag pa)` 
   >| [(* ==> *)
       RW_TAC std_ss [hit_def]
       ,
@@ -371,7 +501,7 @@ val miss_oblg = store_thm("miss_oblg", ``
 
 
 val cdirty_oblg = store_thm("cdirty_oblg", ``
-!pa ca ca'. (ca pa = ca' pa) ==> (cdirty_ ca pa <=> cdirty_ ca' pa)
+!pa ca ca'. (ca (tag pa) = ca' (tag pa)) ==> (cdirty_ ca pa <=> cdirty_ ca' pa)
 ``,
   RW_TAC std_ss [cdirty_def]
 );
@@ -382,11 +512,92 @@ val cdirty_chit_oblg = store_thm("cdirty_chit_oblg", ``
   RW_TAC std_ss [cdirty_def, chit_def, dirty_hit_lem]
 );
 
+val cdirty_other_oblg = store_thm("cdirty_other_oblg", ``
+!ca pa pa'. (tag pa = tag pa') ==> (cdirty_ ca pa <=> cdirty_ ca pa')
+``,
+  RW_TAC std_ss [cdirty_def]
+);
+
+val cdirty_ldirty_oblg = store_thm("cdirty_ldirty_oblg", ``
+!ca pa. cdirty_ ca pa <=> ldirty_ ca (tag pa)
+``,
+  RW_TAC std_ss [cdirty_def, ldirty_def]
+);
+
 val not_chit_not_cdirty_oblg = store_thm("not_chit_not_cdirty_oblg", ``
 !ca pa. ~chit_ ca pa ==> ~cdirty_ ca pa 
 ``,
   RW_TAC std_ss [cdirty_def, chit_def, not_hit_not_dirty_lem]
 );
+
+val lw_ccntw_oblg = store_thm("lw_ccntw_oblg", ``
+!ca pa pa'. (tag pa = tag pa') ==> (lw (ccnt_ ca pa') pa = ccntw_ ca pa)
+``,
+  RW_TAC std_ss [lcnt_def, ccntw_def, ccnt_def]
+);
+
+val lw_lcnt_oblg = store_thm("lw_lcnt_oblg", ``
+!ca pa. lw (lcnt_ ca (tag pa)) pa = ccntw_ ca pa
+``,
+  RW_TAC std_ss [lcnt_def, ccntw_def, ccnt_def]
+);
+
+val lw_lv_oblg = store_thm("lw_lv_oblg", ``
+!mv pa. lw (lv mv T pa) pa = mv T pa
+``,
+  RW_TAC std_ss [lw_def, lv_def, the_line_def]
+);
+
+val lv_oblg = store_thm("lv_oblg", ``
+!mv pa' pa. (tag pa = tag pa') ==> (lv mv T pa' = lv mv T pa)
+``,
+  RW_TAC std_ss [tag_def, lv_def, the_line_def] >>
+  Cases_on `pa` >>
+  Cases_on `pa'` >>
+  FULL_SIMP_TAC std_ss [the_adr_def]
+);
+
+val mllu_lv_oblg = store_thm("mllu_lv_oblg", ``
+!mv m pa pa'. (tag pa = tag pa') ==> 
+    ((lv mv T pa' = mllu m pa) 
+	 <=> 
+     !pa''. (tag pa'' = tag pa) ==> 
+         (lw (lv mv T pa') pa'' = lw (mllu m pa) pa''))
+``,
+  REPEAT STRIP_TAC >>
+  EQ_TAC
+  >| [(* ==> *)
+      REPEAT STRIP_TAC >>
+      RW_TAC std_ss [lw_lv_oblg, mllu_oblg]
+      ,
+      (* <== *)
+      REPEAT STRIP_TAC >>
+      RW_TAC std_ss [lv_def, mllu_def] >>
+      PAT_X_ASSUM ``!pa. x`` (
+          fn thm => ASSUME_TAC ( SPEC ``pa:padr`` thm )
+      ) >>
+      REV_FULL_SIMP_TAC std_ss [] >>
+      Cases_on `pa` >>
+      Cases_on `pa'` >>
+      REV_FULL_SIMP_TAC std_ss [tag_def, the_adr_def] >>
+      FULL_SIMP_TAC std_ss [lw_lv_oblg, mllu_oblg]
+     ]
+); 
+
+val lu_oblg = store_thm("lu_oblg", ``
+!l pa w. lw (lu l pa w) pa = w
+``,
+  RW_TAC std_ss [lw_def, lu_def, the_line_def]
+);
+
+val lu_other_oblg = store_thm("lu_other_oblg", ``
+!l pa w pa'. (tag pa' = tag pa) /\ pa' <> pa ==> (lw (lu l pa w) pa' = lw l pa')
+``,
+  RW_TAC std_ss [tag_def, lw_def, lu_def, the_line_def] >>
+  REV_FULL_SIMP_TAC std_ss [the_adr_inj]
+);
+
+(* transitions *)
 
 val ctf_chit_oblg = store_thm("ctf_chit_oblg", ``
 !ca mv dop ca' y. CA dop /\ ~cl dop /\ ((ca',y) = ctf ca mv dop) ==>
@@ -407,7 +618,7 @@ val ctf_chit_oblg = store_thm("ctf_chit_oblg", ``
 
 val ctf_cl_miss_oblg = store_thm("ctf_cl_miss_oblg", ``
 !ca mv dop ca' y. cl dop /\ ((ca',y) = ctf ca mv dop) ==>
-    ~chit_ ca' (PA dop)
+    !pa. (tag pa = tag (PA dop)) ==> ~chit_ ca' pa
 ``,
   RW_TAC std_ss [] >>
   IMP_RES_TAC cl_CA_lem >>
@@ -417,8 +628,9 @@ val ctf_cl_miss_oblg = store_thm("ctf_cl_miss_oblg", ``
 );
 
 val ctf_cl_other_oblg = store_thm("ctf_cl_other_oblg", ``
-!ca mv dop ca' y pa. cl dop /\ ((ca',y) = ctf ca mv dop) /\ (pa <> PA dop) ==>
-    (ca' pa = ca pa)
+!ca mv dop ca' y pa. cl dop /\ ((ca',y) = ctf ca mv dop) 
+                  /\ (tag pa <> tag (PA dop)) ==>
+    (ca' (tag pa) = ca (tag pa))
 ``,
   RW_TAC std_ss [] >>
   IMP_RES_TAC cl_CA_lem >>
@@ -429,22 +641,22 @@ val ctf_cl_other_oblg = store_thm("ctf_cl_other_oblg", ``
 val ctf_cl_wb_oblg = store_thm("ctf_cl_wb_oblg", ``
 !ca mv dop ca' y pa. cl dop /\ ((ca',y) = ctf ca mv dop) ==>
     (y = if cdirty_ ca (PA dop)
-	 then SOME (PA dop, ccnt_ ca (PA dop))
+	 then SOME (tag (PA dop), ccnt_ ca (PA dop))
 	 else NONE)
 ``,
   RW_TAC std_ss [] >> (
       IMP_RES_TAC cl_CA_lem >>
       FULL_SIMP_TAC std_ss [ctf_lem] >>
-      RW_TAC std_ss [ctf_wb_cl_lem]
+      RW_TAC std_ss [ctf_wb_cl_lem, ccnt_def]
   )
 );
 
 val ctf_not_cl_other_oblg = store_thm("ctf_not_cl_other_oblg", ``
-!ca mv dop ca' y pa. CA dop /\ ~cl dop /\ ((ca',y) = ctf ca mv dop) 
-		  /\ (pa <> PA dop) ==>
-    (ca' pa = if evpol ca (PA dop) = SOME pa 
-	      then NONE
-	      else ca pa)
+!ca mv dop ca' y t. CA dop /\ ~cl dop /\ ((ca',y) = ctf ca mv dop) 
+		  /\ (t <> tag (PA dop)) ==>
+    (ca' t = if evpol ca (PA dop) = SOME t 
+	     then NONE
+	     else ca t)
 ``,
   REPEAT STRIP_TAC >>
   FULL_SIMP_TAC std_ss [not_cl_lem]
@@ -463,10 +675,10 @@ val ctf_not_cl_wb_oblg = store_thm("ctf_not_cl_wb_oblg", ``
 !ca mv dop ca' y. CA dop /\ ~cl dop /\ ((ca',y) = ctf ca mv dop) ==>
     (y = if evpol ca (PA dop) = NONE
 	 then NONE
-	 else (if cdirty_ ca (THE (evpol ca (PA dop))) /\
-	          THE (evpol ca (PA dop)) <> PA dop 
+	 else (if ldirty_ ca (THE (evpol ca (PA dop))) /\
+	          THE (evpol ca (PA dop)) <> tag (PA dop) 
 	       then SOME (THE (evpol ca (PA dop)),
-			  ccnt_ ca (THE (evpol ca (PA dop))))
+			  lcnt_ ca (THE (evpol ca (PA dop))))
 	       else NONE))
 ``,
   REPEAT STRIP_TAC >>
@@ -480,49 +692,95 @@ val ctf_wt_cdirty_oblg = store_thm("ctf_wt_cdirty_oblg", ``
 ``,
   REPEAT STRIP_TAC >>
   REV_FULL_SIMP_TAC std_ss [ctf_lem] >>
-  RW_TAC std_ss [cdirty_def, ctf_ca_wt_lem, dirty_def]
+  RW_TAC std_ss [cdirty_def, ctf_ca_wt_lem, dirty__def]
 );
 
 val ctf_rd_hit_oblg = store_thm("ctf_rd_hit_oblg", ``
 !ca mv dop ca' y. CA dop /\ rd dop /\ chit_ ca (PA dop) 
 	       /\ ((ca',y) = ctf ca mv dop) ==>
-    (ca' (PA dop) = ca (PA dop))
+    (ca' (tag (PA dop)) = ca (tag (PA dop)))
 ``,
   REPEAT STRIP_TAC >>
   REV_FULL_SIMP_TAC std_ss [ctf_lem] >>
-  RW_TAC std_ss [ctf_ca_rd_lem]
+  RW_TAC std_ss [ctf_ca_rd_lem] >>
+  FULL_SIMP_TAC std_ss [chit_def]
 );
 
 val ctf_rd_miss_oblg = store_thm("ctf_rd_miss_oblg", ``
 !ca mv dop ca' y. CA dop /\ rd dop /\ ~chit_ ca (PA dop) 
 	       /\ ((ca',y) = ctf ca mv dop) ==>
     chit_ ca' (PA dop) 
- /\ (ccnt_ ca' (PA dop) = mv T (PA dop))
+ /\ (ccnt_ ca' (PA dop) = lv mv T (PA dop))
+ /\ (ccntw_ ca' (PA dop) = mv T (PA dop))
  /\ ~cdirty_ ca' (PA dop)
 ``,
   REPEAT GEN_TAC >>
-  STRIP_TAC >> STRIP_TAC >>
-  REV_FULL_SIMP_TAC std_ss [ctf_lem] 
-  >| [(* chit *)
+  STRIP_TAC >>
+  REV_FULL_SIMP_TAC std_ss [ctf_lem] >>
+  STRIP_TAC >- (
+      (* chit *)
       RW_TAC std_ss [chit_def, hit_def, ctf_ca_rd_lem]
-      ,
-      (* ccnt and clean *)
-      RW_TAC std_ss [ccnt_def, cnt_def, ctf_ca_rd_lem, not_cdirty_lem]
-     ]      
+  ) >> 
+  STRIP_TAC >- (
+      (* ccnt *)
+      RW_TAC std_ss [ccnt_def, cnt_def, ctf_ca_rd_lem] >>
+      FULL_SIMP_TAC std_ss [chit_def]
+  ) >>
+  STRIP_TAC >- (
+      (* ccntw *)
+      RW_TAC std_ss [ccntw_def, ccnt_def, ctf_ca_rd_lem]
+      >| [(* miss -> contradiction *)
+	  FULL_SIMP_TAC std_ss [chit_def]
+	  ,
+	  (* hit *) 
+	  RW_TAC std_ss [cnt_def, lv_def, lw_def, the_line_def]
+	 ]
+  ) >>
+      (* not_dirty *)
+      RW_TAC std_ss [ctf_ca_rd_lem, not_cdirty_lem] >>
+      FULL_SIMP_TAC std_ss [chit_def]
+);
+
+val ctf_wt_fill_oblg = store_thm("ctf_wt_fill_oblg", ``
+!ca mv dop ca' y pa. CA dop /\ wt dop /\ pa <> PA dop /\ (tag pa = tag (PA dop))
+	          /\ ~chit_ ca (PA dop) /\ ((ca',y) = ctf ca mv dop) ==>
+    chit_ ca' pa 
+ /\ (ccnt_ ca' pa = lv mv T (PA dop))
+``,
+  REPEAT GEN_TAC >>
+  STRIP_TAC >>
+  REV_FULL_SIMP_TAC std_ss [ctf_lem] >>
+  STRIP_TAC >- (
+      (* chit *)
+      RW_TAC std_ss [chit_def, hit_def, ctf_ca_wt_lem]
+  ) >> 
+      (* ccntw *)
+      Cases_on `pa` >>
+      Cases_on `PA dop` >>
+      FULL_SIMP_TAC std_ss [tag_def, the_adr_def]
 );
 
 val ctf_wt_ccnt_oblg = store_thm("ctf_wt_ccnt_oblg", ``
 !ca mv dop ca' y. CA dop /\ wt dop /\ ((ca',y) = ctf ca mv dop) ==>
-    (ccnt_ ca' (PA dop) = VAL dop)
+    (ccntw_ ca' (PA dop) = VAL dop) 
+ /\ (!pa. pa <> PA dop /\ (tag pa = tag (PA dop)) ==> 
+	      (ccntw_ ca' pa = ccntw_ ca pa))
 ``,
-  REPEAT STRIP_TAC >>
+  REPEAT GEN_TAC >> 
+  STRIP_TAC >>
   REV_FULL_SIMP_TAC std_ss [ctf_lem] >>
-  RW_TAC std_ss [ctf_ca_wt_lem, ccnt_def, cnt_def]
+  RW_TAC std_ss [ctf_ca_wt_lem, ccntw_def, ccnt_def, ccntw_def]
+  >| [(* written part *)
+      RW_TAC std_ss [lw_def, cnt_def, the_line_def]
+      ,
+      (* other parts -> contradiction *)
+      FULL_SIMP_TAC std_ss [tag_def, the_adr_inj]
+     ]
 );
 
 val ctf_wb_not_cl_evpol_oblg = store_thm("ctf_wb_not_cl_evpol_oblg", ``
-!ca mv dop ca' pa v. CA dop /\ ~cl dop /\ ((ca',SOME(pa,v)) = ctf ca mv dop) ==>
-    (pa = THE (evpol ca (PA dop))) /\ (v = ccnt_ ca pa) /\ cdirty_ ca pa 
+!ca mv dop ca' t v. CA dop /\ ~cl dop /\ ((ca',SOME(t,v)) = ctf ca mv dop) ==>
+    (t = THE (evpol ca (PA dop))) /\ (v = lcnt_ ca t) /\ ldirty_ ca t 
 ``,
   REPEAT STRIP_TAC >> (
       REV_FULL_SIMP_TAC std_ss [ctf_lem, ctf_wb_not_cl_lem] >>
@@ -532,8 +790,8 @@ val ctf_wb_not_cl_evpol_oblg = store_thm("ctf_wb_not_cl_evpol_oblg", ``
 );
 
 val ctf_wb_not_cl_evpol_some_oblg = store_thm("ctf_wb_not_cl_evpol_some_oblg", ``
-!ca mv dop ca' pa v. CA dop /\ ~cl dop /\ ((ca',SOME(pa,v)) = ctf ca mv dop) ==>
-    (evpol ca (PA dop) = SOME pa)
+!ca mv dop ca' t v. CA dop /\ ~cl dop /\ ((ca',SOME(t,v)) = ctf ca mv dop) ==>
+    (evpol ca (PA dop) = SOME t)
 ``,
   REPEAT STRIP_TAC >> 
   REV_FULL_SIMP_TAC std_ss [ctf_lem, ctf_wb_not_cl_lem] >>
