cache/compile.sh
@@ -1,6 +1,6 @@
 #echo 'val () = Runtime.LoadF"../v8-base_types.spec, ../v8-mem_types.spec, ../v8-seqmem.spec v8-cache-type.spec v8-Dcache.spec v8-cache-base.spec v8-Dcache-base.spec test.spec";val () = SMLExport.export "cache";' | l3
 
-echo 'val () = Runtime.LoadF"v8-cache-type.spec v8-Dcache.spec v8-cache-base.spec test.spec";val () = SMLExport.export "cache";' | l3
+echo 'val () = Runtime.LoadF"v8-cache-type.spec v8-Dcache.spec v8-cache-base.spec";val () = SMLExport.export "cache";' | l3
 #echo 'val () = Runtime.LoadF"v8-cache-type.spec v8-Dcache.spec v8-cache-base.spec";val () = SMLExport.export "cache";' | l3
 
 
